CHERI_Monotonicity.thy
@@ -9,93 +9,6 @@ interpretation Register_Accessors get_regval set_regval
   apply standard
   sorry
 
-definition "determ_instrs_of_exp m \<equiv>
-  (\<forall>t. hasTrace t m \<longrightarrow> instrs_of_exp m = set_option (instr_of_trace t))"
-
-lemma hasTrace_determ_instrs_eqs:
-  assumes "hasTrace t m" and "determ_instrs_of_exp m"
-  shows "exp_invokes_regs m = trace_invokes_regs t"
-    and "exp_invokes_indirect_regs m = trace_invokes_indirect_regs t"
-    and "exp_load_auths m = trace_load_auths t"
-    and "exp_is_indirect_branch m = trace_is_indirect_branch t"
-  using assms
-  unfolding exp_invokes_regs_def trace_invokes_regs_def
-  unfolding exp_invokes_indirect_regs_def trace_invokes_indirect_regs_def
-  unfolding exp_load_auths_def trace_load_auths_def
-  unfolding trace_is_indirect_branch_def
-  by (auto simp: determ_instrs_of_exp_def split: option.splits)
-
-lemma determ_instrs_instr_sem: "determ_instrs_of_exp (instr_sem instr)"
-  sorry
-
-lemma trace_invokes_indirect_regs_None[simp]:
-  assumes "instr_of_trace t = None"
-  shows "trace_invokes_indirect_regs t = {}"
-  using assms
-  by (auto simp: trace_invokes_indirect_regs_def)
-
-lemma instr_trace_invokes_indirect_regs[simp]:
-  assumes "instr_of_trace t = Some instr"
-  shows "trace_invokes_indirect_regs t = instr_invokes_indirect_regs instr"
-  using assms
-  by (auto simp: trace_invokes_indirect_regs_def)
-
-lemma trace_invokes_indirect_caps_no_regs[simp]:
-  assumes "trace_invokes_indirect_regs t = {}"
-  shows "trace_invokes_indirect_caps t = {}"
-  using assms
-  by (auto simp: trace_invokes_indirect_caps_def)
-
-context Morello_Axiom_Automaton
-begin
-
-lemma instrs_eq_instr_exp_assms_iff:
-  assumes "instrs_of_exp m1 = instrs_of_exp m2"
-  shows "instr_exp_assms m1 \<longleftrightarrow> instr_exp_assms m2"
-  using assms
-  unfolding instr_exp_assms_def invocation_instr_exp_assms_def load_instr_exp_assms_def
-  unfolding exp_invokes_regs_def exp_invokes_indirect_regs_def exp_load_auths_def
-  by auto
-
-lemma T_bind_leftI:
-  assumes "(m, e, m') \<in> T"
-  shows "(bind m f, e, bind m' f) \<in> T"
-  using assms
-  by induction auto
-
-lemma Traces_bind_leftI:
-  assumes "(m, t, m') \<in> Traces"
-  shows "(bind m f, t, bind m' f) \<in> Traces"
-  using assms
-  by induction (auto intro: T_bind_leftI)
-
-lemma instr_of_trace_no_writes_None:
-  assumes "\<nexists>v. E_write_reg ''__ThisInstrAbstract'' v \<in> set t"
-  shows "instr_of_trace t = None"
-  using assms
-  by (cases t rule: instr_of_trace.cases) auto
-
-lemma instr_of_trace_append_no_writes:
-  assumes "\<nexists>v. E_write_reg ''__ThisInstrAbstract'' v \<in> set t2"
-  shows "instr_of_trace (t1 @ t2) = instr_of_trace t1"
-  using assms
-  by (cases t1 rule: instr_of_trace.cases) (auto simp: instr_of_trace_no_writes_None)
-
-lemma instrs_of_exp_bind_no_writes:
-  assumes "\<forall>a. no_reg_writes_to {''__ThisInstrAbstract''} (f a)"
-  shows "instrs_of_exp (bind m f) = instrs_of_exp m"
-  using assms
-  by (fastforce simp: instrs_of_exp_def instr_of_trace_append_no_writes no_reg_writes_to_def
-                intro: Traces_bind_leftI elim!: bind_Traces_cases)
-
-lemma instr_exp_assms_TryInstructionExecute_iff:
-  "instr_exp_assms (TryInstructionExecute enc instr) \<longleftrightarrow> instr_exp_assms (DecodeExecute enc instr)"
-  unfolding TryInstructionExecute_def SSAdvance_def bind_assoc
-  by (intro instrs_eq_instr_exp_assms_iff instrs_of_exp_bind_no_writes allI)
-     (no_reg_writes_toI simp: register_defs)
-
-end
-
 locale Morello_Trace_Automaton = Morello_Fixed_Address_Translation + fixes t :: "register_value trace"
 
 locale Morello_Instr_Trace_Automaton = Morello_Trace_Automaton + fixes instr :: instr
@@ -188,15 +101,8 @@ locale Morello_Fetch_Trace_Mem_Automaton =
     and no_system_reg_access = "\<not>trace_has_system_reg_access t"
     and is_in_c64 = "trace_is_in_c64 t"
 
-term Morello_Instr_Trace_Write_Cap_Automaton.instr_trace_assms
-
 context Morello_Fixed_Address_Translation
 begin
-
-thm Morello_Axiom_Assms.ev_assms.simps
-term "Morello_Instr_Trace_Write_Cap_Automaton.instr_trace_assms translate_address is_translation_event translation_assms UNKNOWN_caps"
-
-abbreviation "instr_ev_assms_in_trace instr t \<equiv> Morello_Axiom_Assms.ev_assms UNKNOWN_caps (invokes_caps instr t) (trace_invokes_regs t) (trace_invokes_indirect_caps t) (trace_invokes_indirect_regs t) (trace_load_auths t) (trace_uses_mem_caps t) False (trace_is_indirect_branch t) (\<not>trace_has_system_reg_access t) (trace_is_in_c64 t) translation_assms"
 
 abbreviation "instr_assms instr t \<equiv> Morello_Instr_Trace_Write_Cap_Automaton.instr_trace_assms translate_address is_translation_event translation_assms UNKNOWN_caps t"
 abbreviation "fetch_assms t \<equiv> Morello_Fetch_Trace_Write_Cap_Automaton.fetch_trace_assms translate_address is_translation_event translation_assms UNKNOWN_caps t"
@@ -206,10 +112,9 @@ lemma more_ISA_simps[simp]:
   by (auto simp: ISA_def)
 
 (* TODO:
-   - Add write_reg_axiom to traces_enabled_reg_axioms
-   - Add hasFailure to fetch_raises_ex
    - Later: Restrict ex_traces case to only exceptions, not failures; clean up instr/fetch_raises_ex again
-   - Add __FetchNextInstr and __CheckPendingInterrupts to fetch exps in lemma generation
+   - Move translate_address_aligned_iff to Morello_Fixed_Address_Translation
+   - Move no_reg_writes_to lemmas outisde of context (to speed up interpretation)
  *)
 
 sublocale CHERI_ISA CC ISA cap_invariant UNKNOWN_caps fetch_assms instr_assms
@@ -226,45 +131,18 @@ proof
   from ia have no_asr: "\<not>trace_has_system_reg_access t"
     by simp
   have *: "Write_Cap.traces_enabled (instr_sem instr) initial"
-    unfolding instr_sem_def TryInstructionExecute_def bind_assoc
-    by (traces_enabledI assms: iea simp: instr_sem_def instr_exp_assms_TryInstructionExecute_iff
-          intro: no_asr elim: BranchTaken_or_PCC_accessible)
+    unfolding instr_sem_def
+    by (traces_enabledI assms: iea simp: instr_sem_def intro: no_asr)
   interpret Mem: Morello_Instr_Trace_Mem_Automaton where instr = instr and t = t
     by standard (auto simp: trace_uses_mem_caps_def)
   have **: "Mem.traces_enabled (instr_sem instr) initial"
     unfolding instr_sem_def TryInstructionExecute_def bind_assoc
     by (traces_enabledI assms: iea simp: instr_sem_def instr_exp_assms_TryInstructionExecute_iff intro: no_asr)
   show "instr_cheri_axioms instr t n"
-    using * **
+    using * ** t inv ia n
     unfolding cheri_axioms_def ISA_simps
-    apply (intro conjI)
-    subgoal
-      apply (elim traces_enabled_reg_axioms)
-      using t inv ia n
-      by (auto simp: instr_raises_ex_def intro: holds_along_trace_take)
-    subgoal
-      apply (elim traces_enabled_reg_axioms)
-      using t inv ia n
-      by (auto simp: instr_raises_ex_def intro: holds_along_trace_take)
-    subgoal
-      apply (elim traces_enabled_reg_axioms)
-      using t inv ia n
-      by (auto simp: instr_raises_ex_def intro: holds_along_trace_take)
-    subgoal
-      sorry
-    subgoal
-      apply (elim Mem.traces_enabled_mem_axioms)
-      using t inv ia n
-      by (auto simp: instr_raises_ex_def intro: holds_along_trace_take)
-    subgoal
-      apply (elim Mem.traces_enabled_mem_axioms)
-      using t inv ia n
-      by (auto simp: instr_raises_ex_def intro: holds_along_trace_take)
-    subgoal
-      apply (elim Mem.traces_enabled_mem_axioms)
-      using t inv ia n
-      by (auto simp: instr_raises_ex_def intro: holds_along_trace_take)
-    done
+    by (intro conjI; elim traces_enabled_reg_axioms Mem.traces_enabled_mem_axioms)
+       (auto simp: instr_raises_ex_def intro: holds_along_trace_take)
 next
   fix t :: "register_value trace" and n :: nat
   interpret Write_Cap?: Morello_Fetch_Trace_Write_Cap_Automaton where t = t
@@ -276,65 +154,37 @@ next
   from ia have no_asr: "\<not>trace_has_system_reg_access t"
     by simp
   have *: "Write_Cap.traces_enabled (instr_fetch) initial"
-    unfolding instr_fetch_def FetchNextInstr_def bind_assoc
-    apply (traces_enabledI)
-    sorry
+    unfolding instr_fetch_def bind_assoc
+    by traces_enabledI
   interpret Mem: Morello_Fetch_Trace_Mem_Automaton where t = t
     by standard auto
   have **: "Mem.traces_enabled (instr_fetch) initial"
-    unfolding instr_fetch_def FetchNextInstr_def bind_assoc
-    apply (traces_enabledI)
-    sorry
+    unfolding instr_fetch_def bind_assoc
+    by traces_enabledI
   show "fetch_cheri_axioms t n"
-    using * **
+    using * ** t inv ia n
     unfolding cheri_axioms_def ISA_simps more_ISA_simps
-    apply (intro conjI)
-    subgoal
-      apply (elim traces_enabled_reg_axioms)
-      using t inv ia n
-      apply (auto simp: fetch_raises_ex_def intro: holds_along_trace_take)
-      sorry
-    subgoal
-      apply (elim traces_enabled_reg_axioms)
-      using t inv ia n
-      apply (auto simp: fetch_raises_ex_def intro: holds_along_trace_take)
-      sorry
-    subgoal
-      apply (elim traces_enabled_reg_axioms)
-      using t inv ia n
-      apply (auto simp: fetch_raises_ex_def intro: holds_along_trace_take)
-      sorry
-    subgoal
-      sorry
-    subgoal
-      apply (elim Mem.traces_enabled_mem_axioms)
-      using t inv ia n
-      apply (auto simp: fetch_raises_ex_def intro: holds_along_trace_take)
-      sorry
-    subgoal
-      apply (elim Mem.traces_enabled_mem_axioms)
-      using t inv ia n
-      apply (auto simp: fetch_raises_ex_def intro: holds_along_trace_take)
-      sorry
-    subgoal
-      apply (elim Mem.traces_enabled_mem_axioms)
-      using t inv ia n
-      apply (auto simp: fetch_raises_ex_def intro: holds_along_trace_take)
-      sorry
-    done
+    by (intro conjI; elim traces_enabled_reg_axioms Mem.traces_enabled_mem_axioms)
+       (auto simp: fetch_raises_ex_def intro: holds_along_trace_take)
 qed
 
-(*abbreviation "s_translate_address addr acctype s \<equiv> translate_address addr"
+abbreviation "s_translate_address addr acctype s \<equiv> translate_address addr"
 
 sublocale CHERI_ISA_State CC ISA cap_invariant UNKNOWN_caps fetch_assms instr_assms get_regval set_regval s_translate_address
-  apply standard
-  subgoal
-    apply (auto simp: set_regval_unfold get_regval_unfold split: bind_splits)
+proof
+  fix t s vaddr paddr load
+  assume "s_allows_trace t s" and "isa.translate_address ISA vaddr load t = Some paddr"
+  then show "translate_address vaddr = Some paddr"
+    by (auto simp: ISA_def)
+next
+  fix s vaddr paddr load
+  assume "translate_address vaddr = Some paddr"
+  then show "address_tag_aligned ISA paddr = address_tag_aligned ISA vaddr"
+    thm Morello_Mem_Axiom_Automaton.translate_address_aligned_iff
     sorry
-  subgoal
-    apply (auto simp: set_regval_unfold get_regval_unfold split: bind_splits)
-    sorry
-  sorry*)
+qed
+
+thm reachable_caps_instrs_trace_intradomain_monotonicity
 
 end
 
